Explicited explode example

ulib/experimental/Steel.Extracted.ArrayStruct.fsti
@@ -26,6 +26,7 @@ open FStar.FunctionalExtensionality
 module PCM = Steel.PCM
 module UPCM = Steel.PCM.Unitless
 module UPCMBase = Steel.PCM.Unitless.Base
+module PCMBase = Steel.PCM.Base
 
 open Steel.PCM.Effect
 open Steel.PCM.Memory
@@ -47,8 +48,6 @@ type low_foo = {
 
 val foo_to_low_foo : foo -> low_foo
 
-val low_foo_to_foo : low_foo -> foo
-
 (* The representation of the objects managed by [foo_pcm] in memory is low_foo *)
 (* [@@repr [low_foo, foo_to_low_foo, low_foo_to_foo]] *)
 val foo_pcm : PCM.pcm foo
@@ -58,14 +57,20 @@ class low_level_type (a: Type u#a) = {
   pcm: PCM.pcm a;
   low_a: Type u#a;
   a_to_low_a: a -> low_a;
-  low_a_to_a: low_a -> a
 }
+
+(* Check by tactic that [low_a] corresponds to something like Steel.PCM.ArrayStruct.descriptor *)
+
+(*
+  Second tactic : if [a] is already in the [low_a] format, then have a tactic that metaprograms
+  all the getters and setters.
+  Future work, only after we have a working setup
+*)
 
 instance low_level_foo : low_level_type foo = {
   pcm = foo_pcm;
   low_a = low_foo;
   a_to_low_a = foo_to_low_foo;
-  low_a_to_a = low_foo_to_foo;
 }
 
 open FStar.Tactics.Typeclasses
@@ -91,14 +96,28 @@ let main () =
 
 (* You have to give update_z because you have to justify this with regards to [foo_pcm] *)
 
-(*  [@@ update low_foo.z] (* What checks for this attribute ?
+
+val update: unit -> Tot unit
+val get: unit -> Tot unit
+val focus: unit -> Tot unit
+val explode: unit -> Tot unit
+val op_String_Access : unit -> Tot unit
+
+open FStar.Tactics
+
+let check (src: string) : Tac unit =
+  let _ = lookup_typ (top_env ()) (cur_module () @ [ src ]) in
+  exact (`(()))
+
+(* What checks for this attribute ?
     - number of arguments: 2
     - first argument is ref to type that has low_level_type typeclass
     - [low_foo] is [low_a] for that typeclass
     - z is a field of low_foo (low_foo has to be a record)
     - postcondition implies that (a_to_low_a (sel h1 r))  == { a_to_low_a (sel h0 r) with z = new_val }
-  *) *)
-  val update_z (r: ref foo) (new_val: UInt64.t)
+  *)
+[@@ update low_foo.z]
+val update_z (r: ref foo) (new_val: UInt64.t)
     : Steel unit (admit(); ref_hprop r) (fun _ -> ref_hprop r)
     (fun h0 ->
       UInt64.v new_val >= UInt32.v (sel h0 r).x + UInt32.v (sel h0 r).y
@@ -106,10 +125,90 @@ let main () =
       (sel h1 r) = MkFoo (sel h0 r).x (sel h0 r).y new_val
     )
 
+let _ : unit  = _ by (check (`%update_z))
+
+(* What does this attribute check ?
+    - number of arguments: 2
+    - first argument is ref to type that has low_level_type typeclass
+    - [low_foo] is [low_a] for that typeclass
+    - .x.[0] is a subpath of low_foo
+    - postcondition (fun h0 x h1) implies that (
+      a_to_low_a (sel h0 r) == a_to_low_a (sel h1 r) /\
+      x == a_to_low_a (sel h1 r).x.[0]
+     )
+*)
+[@@get low_foo.x.[0]]
+val get_x (r: ref foo) : Steel (UInt32.t) (admit(); ref_hprop r) (fun _ -> ref_hprop r)
+  (fun _ -> True) (fun h0 x h1 ->
+    sel h0 r == sel h1 r /\ x == (sel h1 r).x
+  )
+
 (* Language of attributes :
    [@@ update low_struct.field]
    [@@ update low_array.index] and paths thereof
    [@@ read low_struct.field]
    [@@ read low_array.index] and paths thereof
-   [@@ address_of low_struct.field]
+   [@@ focus low_struct.field -> field_low]
+   [@@ explode low_struct -> [field1_low; field2_low]]
 *)
+
+val u32_pcm : PCM.pcm UInt32.t
+
+instance low_level_x : low_level_type UInt32.t = {
+  pcm = u32_pcm;
+  low_a = UInt32.t;
+  a_to_low_a = (fun (x: UInt32.t) -> x);
+}
+
+
+/// Ok we have getters and setters. But what about addresses ? We need:
+/// - a type for the sub-object that you want to take address
+/// - a PCM governing the values of the sub-object
+/// - a magic_wand to focus on the sub-object
+/// - an explode operation that explodes a parent object into multiple sub-objects
+
+
+(* This yields a magic wand in the function's signature. Things checked by the attribute:
+    - number of arguments: 1
+    - first argument is ref to type that has low_level_type typeclass
+    - [low_foo] is [low_a] for that typeclass
+    - x.[0] is a subpath of low_foo
+    - return type is ref to type that has the second low_level_type typeclass
+    - postcondition implies
+      a_to_low_a (sel h0 r) == a_to_low_a (sel h1 r) /\ (sel h1 r') == (sel h0 r).x
+*)
+[@@focus low_foo.x.[0] -> low_level_x]
+val focus_x (r: ref foo) : Steel (ref UInt32.t) (admit();ref_hprop r) (fun r' ->
+   ref_hprop r' `star`
+   wand (ref_hprop r') (ref_hprop r)
+ ) (fun _ -> True) (fun h0 r' h1 ->
+   (sel h0 r) == (sel h1 r) /\ (sel h1 r') == (sel h0 r).x
+ )
+
+val u64_pcm : PCM.pcm UInt64.t
+
+instance low_level_z : low_level_type UInt64.t = {
+  pcm = u64_pcm;
+  low_a = UInt64.t;
+  a_to_low_a = (fun x -> x);
+}
+
+val xy_pcm : PCM.pcm (Seq.lseq UInt32.t 2)
+
+instance low_level_xy : low_level_type (Seq.lseq UInt32.t 2) = {
+  pcm = xy_pcm;
+  low_a = (Seq.lseq UInt32.t 2);
+  a_to_low_a = (fun x -> x);
+}
+
+(* This yields the totality of the parent object but exploded in slprops *)
+[@@explode low_foo -> (low_level_xy, low_level_z)]
+val explode_xy_z (r: ref foo)
+  : Steel (admit();(ref (Seq.lseq UInt32.t 2) #low_level_xy & ref UInt64.t))
+  (ref_hprop r) (fun (r1, r2) -> ref_hprop r1 `star` ref_hprop r2)
+  (fun _ -> True)
+  (fun h0 (r1, r2) h1 ->
+    Seq.index (sel h1 r1) 0 == MkFoo?.x (sel h0 r) /\
+    Seq.index (sel h1 r1) 1 == (sel h0 r).y /\
+    sel h1 r2 == MkFoo?.z (sel h0 r)
+  )
